crdt_specs_v.thy
@@ -1,0 +1,241 @@
+section "CRDT Specifications For Verification"
+theory crdt_specs_v
+  imports repliss_sem crdt_specs
+begin
+
+
+text "The previous CRDT are not nice to work with when composed.
+The problem is, that the specifications for maps and structs transform the context
+passed to embedded CRDTs.
+During this transformation the reverse direction is lost, so it is hard to reconstruct the original
+calls from the calls in an embedded context.
+Therefore, we now use a different composition technique, where the mapping is explicitly passed down
+into nested CRDTs."
+
+text "In the following type definition we have three type parameters:
+
+\<^enum> op is the type of operations at the top level
+\<^enum> opn is the type of nested operations, on which the specification works
+\<^enum> res is the type of results "
+
+type_synonym ('op, 'opn, 'res) cOperationResultSpec = 
+        "callId set                  \<comment> \<open>visible calls\<close>
+      \<Rightarrow> (callId \<Rightarrow>'op)              \<comment> \<open>call information\<close> 
+      \<Rightarrow> callId rel                  \<comment> \<open>happens-before\<close>
+      \<Rightarrow> ('opn \<Rightarrow> 'op)               \<comment> \<open>mapping back\<close>
+      \<Rightarrow> 'res
+      \<Rightarrow> bool"
+
+type_synonym ('op, 'opn, 'res) ccrdtSpec = 
+        "'opn \<Rightarrow> ('op, 'opn, 'res) cOperationResultSpec"
+
+
+definition 
+"extract_op c_calls c \<equiv> call_operation (the (c_calls c))"
+
+text "The following function converts "
+
+definition toplevel_spec :: "('op, 'op, 'res) ccrdtSpec \<Rightarrow>  ('op, 'res, 'a) operationContext_scheme \<Rightarrow> callId set \<Rightarrow> 'op \<Rightarrow> 'res  \<Rightarrow> bool" where
+"toplevel_spec S ctxt vis op  \<equiv> S op vis (extract_op (calls ctxt)) (happensBefore ctxt) id"
+
+
+
+
+text "There is a mapping between the composable CRDT specs above and the original specifications:"
+
+
+
+lemma extract_op_def':
+"extract_op (c_calls::('b \<Rightarrow> ('a, 'c) call option)) c 
+  = ( case c_calls c of Some (Call op r) \<Rightarrow> op | _ \<Rightarrow> call_operation (the (None :: ('a, 'c) call option)))"
+  by (auto simp add: extract_op_def split: option.splits call.splits) 
+
+
+lemma extract_op_eq:
+  assumes "c\<in>dom c_calls"
+  shows "extract_op c_calls c = oper \<longleftrightarrow> (\<exists>res. c_calls c \<triangleq> Call oper res)"
+  using assms by (auto simp add: extract_op_def' split: option.splits call.splits)
+
+
+
+
+lemma calls_sub_context:
+  "calls (sub_context C_in Cs ctxt) = 
+(\<lambda>c. (calls ctxt |` Cs) c \<bind> (\<lambda>call. case C_in (call_operation call) of None \<Rightarrow> None | Some op' \<Rightarrow> Some (Call op' (call_res call))))
+"
+  by (auto simp add: sub_context_def restrict_ctxt_op_def restrict_ctxt_def fmap_map_values_def ctxt_restrict_calls_def 
+      option_bind_def 
+      split: option.splits call.splits)
+
+lemma happens_before_sub_context:
+  "(x,y) \<in> happensBefore (sub_context C_in Cs ctxt) 
+\<longleftrightarrow> ((x,y) \<in> happensBefore ctxt \<and> x\<in>dom (calls (sub_context  C_in Cs ctxt)) \<and> y\<in>dom (calls (sub_context  C_in Cs ctxt)))
+"
+  by (auto simp add: sub_context_def restrict_ctxt_op_def restrict_ctxt_def fmap_map_values_def
+ ctxt_restrict_calls_def restrict_map_def restrict_relation_def option_bind_def 
+ split: if_splits option.splits call.splits)
+
+
+lemma dom_calls_sub_context_rewrite: "(dom (map_map (calls ctxt) call_operation \<ggreater> C_in) \<inter> Cs)
+  = (dom (calls (sub_context C_in Cs ctxt)))"
+  by (auto simp add: calls_sub_context option_bind_def map_chain_def restrict_map_def  split: option.splits if_splits)
+
+
+
+lemma extract_op_to_call:
+  assumes "is_reverse C_in C_out"
+and "c\<in>dom (calls (sub_context C_in Cs ctxt))"
+shows "extract_op (calls ctxt) c = C_out op
+\<longleftrightarrow> (\<exists>r. calls ctxt c \<triangleq> Call (C_out op) r)"
+  by (smt IntD2 assms(2) call.collapse call.sel(1) calls_sub_context domExists_simp domIff dom_calls_sub_context_rewrite extract_op_def is_none_bind is_none_simps(1) is_none_simps(2) option.sel restrict_in)
+
+lemma extract_op_into_sub_context:
+  assumes is_rev: "is_reverse C_in C_out"
+and in_dom: "c\<in>dom (calls (sub_context C_in Cs ctxt))"
+shows "extract_op (calls ctxt) c = C_out op
+\<longleftrightarrow> (\<exists>r. calls (sub_context C_in Cs ctxt) c \<triangleq> Call op r)"
+  using in_dom  apply (auto simp add: calls_sub_context restrict_map_def option_bind_def
+ call_operation_def extract_op_def is_rev is_reverse_2
+      split: option.splits if_splits call.splits)
+  using is_rev is_reverse_1 by fastforce
+
+lemma happens_before_into_sub_context:
+  assumes is_rev: "is_reverse C_in C_out"
+and in_dom_x: "x\<in>dom (calls (sub_context C_in Cs ctxt))"
+and in_dom_y: "y\<in>dom (calls (sub_context C_in Cs ctxt))"
+shows "(x,y) \<in> happensBefore ctxt
+\<longleftrightarrow> (x,y) \<in> happensBefore (sub_context C_in Cs ctxt)"
+  using in_dom_x in_dom_y  by (auto simp add:  restrict_map_def option_bind_def
+ call_operation_def extract_op_def is_rev is_reverse_2
+ happens_before_sub_context
+      split: option.splits if_splits call.splits)
+
+
+
+definition crdt_spec_rel :: "('opn, 'res) crdtSpec \<Rightarrow> ('op, 'opn, 'res) ccrdtSpec \<Rightarrow> bool" where
+"crdt_spec_rel spec cspec \<equiv>
+\<forall>C_in::'op \<rightharpoonup> 'opn. \<forall>C_out::'opn \<Rightarrow> 'op.
+  is_reverse C_in C_out
+  \<longrightarrow> 
+  (\<forall>ctxt (outer_op::'op) (op::'opn) r Cs. 
+       C_in outer_op \<triangleq> op
+    \<longrightarrow> Cs \<subseteq> (dom ((map_map (calls ctxt) call_operation) \<ggreater> C_in))
+    \<longrightarrow> operationContext_wf ctxt
+    \<longrightarrow>
+       (spec op (sub_context C_in Cs ctxt) r
+    \<longleftrightarrow> cspec op Cs (extract_op (calls ctxt))  (happensBefore ctxt) C_out r))
+
+"
+
+lemmas use_crdt_spec_rel = crdt_spec_rel_def[unfolded atomize_eq, THEN iffD1, rule_format]
+lemmas use_crdt_spec_rel1 = crdt_spec_rel_def[unfolded atomize_eq, THEN iffD1, rule_format, THEN iffD1]
+lemmas use_crdt_spec_rel2 = crdt_spec_rel_def[unfolded atomize_eq, THEN iffD1, rule_format, THEN iffD2]
+
+lemma use_crdt_spec_rel_toplevel:
+  assumes rel: "crdt_spec_rel spec cspec"
+    and hb_wf: "Field (happensBefore ctxt) \<subseteq> dom (calls ctxt)"
+    and "operationContext_wf ctxt"
+  shows "spec op ctxt r 
+ =  cspec op (dom (calls ctxt)) (extract_op (calls ctxt)) (happensBefore ctxt) id  r"
+proof (fuzzy_rule use_crdt_spec_rel[OF rel])
+  show "is_reverse Some id"
+    by (simp add: is_reverse_def)
+
+  show "Some op \<triangleq> op"
+    by simp
+
+  show "dom (calls ctxt) \<subseteq> dom (map_map (calls ctxt) call_operation \<ggreater> Some)"
+    by (auto simp add: dom_map_map dom_map_chain)
+
+  have h1: "calls (sub_context Some UNIV ctxt) =  calls ctxt "
+    by (auto simp add: calls_sub_context)
+
+  have h2: "happensBefore (sub_context Some UNIV ctxt) =  happensBefore ctxt "
+    apply (auto simp add: happens_before_sub_context calls_sub_context)
+     apply (meson FieldI1 domD hb_wf subsetD)
+    by (meson FieldI2 domD hb_wf in_mono)
+
+
+  from h1 h2
+  show "sub_context Some (dom (calls ctxt)) ctxt = ctxt"
+    by (simp add: ctxt_restrict_calls_def hb_wf restrict_map_noop restrict_relation_noop sub_context_def)
+
+  show "operationContext_wf ctxt" using `operationContext_wf ctxt` .
+qed
+
+
+
+lemma show_crdt_spec_rel:
+  assumes
+  a: "\<And>C_in C_out  ctxt outer_op op r Cs.
+\<lbrakk>is_reverse C_in C_out; 
+operationContext_wf ctxt;
+ C_in outer_op \<triangleq> op\<rbrakk> \<Longrightarrow>
+     spec op (sub_context C_in Cs ctxt) r
+ \<longleftrightarrow> cspec op (dom (calls (sub_context C_in Cs ctxt))) (extract_op (calls ctxt))  (happensBefore ctxt) C_out  r 
+"
+shows "crdt_spec_rel spec cspec"
+  by (simp add: crdt_spec_rel_def assms dom_calls_sub_context_rewrite inf.absorb_iff2)
+
+
+definition convert_spec ::  "('op, 'op, 'res) ccrdtSpec \<Rightarrow> ('op, 'res) crdtSpec" where
+"convert_spec cspec op ctxt res \<equiv> 
+  cspec op (dom (calls ctxt)) (extract_op (calls ctxt)) (happensBefore ctxt) id  res"
+
+
+lemma crdt_spec_rel_convert:
+  assumes rel: "crdt_spec_rel spec cspec"
+    and field: "Field (happensBefore ctxt) \<subseteq> dom (calls (ctxt))"
+    and "operationContext_wf ctxt"
+  shows "spec op ctxt r = convert_spec cspec op ctxt r"
+  unfolding convert_spec_def
+proof -
+  show "spec op ctxt r = cspec op (dom (calls ctxt)) (extract_op (calls ctxt)) (happensBefore ctxt) id  r" 
+  proof (fuzzy_rule use_crdt_spec_rel[OF rel])
+    show "is_reverse Some id"
+      by (simp add: is_reverse_def)
+    show "Some op \<triangleq> op"
+      by simp
+    show "dom (calls ctxt) \<subseteq> dom (map_map (calls ctxt) call_operation \<ggreater> Some)"
+      by (auto simp add: map_chain_def)
+    have h1: "calls (sub_context Some UNIV ctxt) = calls ctxt "
+      by (auto simp add: calls_sub_context)
+
+    have h2: "happensBefore (sub_context Some UNIV ctxt) = happensBefore ctxt "
+      using field by (auto simp add: happens_before_sub_context
+          FieldI1 FieldI2 h1 domD subset_h1)
+
+    from h1 h2
+    show "sub_context Some (dom (calls ctxt)) ctxt = ctxt"
+      by (simp add: ctxt_restrict_calls_def field restrict_map_noop restrict_relation_noop sub_context_def)
+
+
+    show "operationContext_wf ctxt"
+      by (simp add: assms)
+  qed
+qed
+
+
+
+definition ccrdtSpec_wf :: "('op, 'opn, 'res) cOperationResultSpec \<Rightarrow> bool" where
+"ccrdtSpec_wf spec  \<equiv> 
+\<forall>Cs op op' hb hb' C_out r. 
+map_same_on Cs op op'
+\<longrightarrow> rel_same_on Cs hb hb'
+\<longrightarrow> (     spec Cs op  hb  C_out r 
+     \<longleftrightarrow>  spec Cs op' hb' C_out r)"
+
+
+
+lemmas use_ccrdtSpec_wf = ccrdtSpec_wf_def[unfolded atomize_eq, THEN iffD1, rule_format]
+lemmas use_ccrdtSpec_wf1 = ccrdtSpec_wf_def[unfolded atomize_eq, THEN iffD1, rule_format, THEN iffD1]
+lemmas use_ccrdtSpec_wf2 = ccrdtSpec_wf_def[unfolded atomize_eq, THEN iffD1, rule_format, THEN iffD2]
+
+
+lemma ccrdtSpec_wf_split_ops:
+  assumes "\<And>x. ccrdtSpec_wf (\<lambda>i. f x)"
+  shows "ccrdtSpec_wf f"
+  using assms by (auto simp add: ccrdtSpec_wf_def)
+
+
+end
